Add a construct to use expressions of Option types
Modify the type system to enforce type-wellformedness and modify the type soundness proofs accordingly

fiat2/src/fiat2/Examples.v
@@ -25,6 +25,7 @@ Section fold_expr.
       | EInsert d k v => EInsert (fold_expr d) (fold_expr k) (fold_expr v)
       | EDelete d k => EDelete (fold_expr d) (fold_expr k)
       | ELookup d k => ELookup (fold_expr d) (fold_expr k)
+      | EOptmatch e e_none x e_some => EOptmatch (fold_expr e) (fold_expr e_none) x (fold_expr e_some)
       | EFilter e x p => EFilter (fold_expr e) x (fold_expr p)
       | EJoin e1 e2 x y p r => EJoin (fold_expr e1) (fold_expr e2) x y (fold_expr p) (fold_expr r)
       | EProj e x r => EProj (fold_expr e) x (fold_expr r)
@@ -71,25 +72,26 @@ Section Examples.
     reflexivity. Abort.
 
   Definition typed_ex1 := synthesize_expr map.empty map.empty ex1.
-  Compute typed_ex1.
-  Compute (fold_expr to_filter_head ex1).
+  (* Compute typed_ex1.
+  Compute (fold_expr to_filter_head ex1). *)
 
   Fixpoint free_immut_in (x : string) (e : expr) : bool :=
     match e with
     | EVar y => String.eqb x y
     | ELoc _ | EAtom _ => false
     | EUnop _ e => free_immut_in x e
-    | EBinop _ e1 e2 => (free_immut_in x e1) || (free_immut_in x e2)
-    | EIf e1 e2 e3 => (free_immut_in x e1) || (free_immut_in x e2) || (free_immut_in x e3)
-    | ELet e1 y e2 | EFlatmap e1 y e2 => (free_immut_in x e1) || (negb (String.eqb x y) && free_immut_in x e2)
-    | EFold e1 e2 y z e3 => (free_immut_in x e1) || (free_immut_in x e2) || (negb (String.eqb x y) && negb (String.eqb x z) && free_immut_in x e3)
+    | EBinop _ e1 e2 => free_immut_in x e1 || free_immut_in x e2
+    | EIf e1 e2 e3 => free_immut_in x e1 || free_immut_in x e2 || free_immut_in x e3
+    | ELet e1 y e2 | EFlatmap e1 y e2 => free_immut_in x e1 || (negb (String.eqb x y) && free_immut_in x e2)
+    | EFold e1 e2 y z e3 => free_immut_in x e1 || free_immut_in x e2 || (negb (String.eqb x y) && negb (String.eqb x z) && free_immut_in x e3)
     | ERecord l => existsb (fun '(_, e) => free_immut_in x e) l
     | EAccess e _ => free_immut_in x e
     | EDict l => existsb (fun '(e1, e2) => orb (free_immut_in x e1) (free_immut_in x e2)) l
-    | EInsert d k v => (free_immut_in x d) || (free_immut_in x k) || (free_immut_in x v)
-    | EDelete d k | ELookup d k => (free_immut_in x d) || (free_immut_in x k)
+    | EInsert d k v => free_immut_in x d || free_immut_in x k || free_immut_in x v
+    | EDelete d k | ELookup d k => free_immut_in x d || free_immut_in x k
+    | EOptmatch e e_none y e_some => free_immut_in x e || free_immut_in x e_none || (negb (String.eqb x y) && free_immut_in x e_some)
     | EFilter e y p => free_immut_in x e || (negb (String.eqb x y) && free_immut_in x p)
-    | EJoin e1 e2 x1 x2 p r => (free_immut_in x e1) || (free_immut_in x e2) ||
+    | EJoin e1 e2 x1 x2 p r => free_immut_in x e1 || free_immut_in x e2 ||
                                  (negb (String.eqb x x1) && negb (String.eqb x x2) && (free_immut_in x p || free_immut_in x r))
     | EProj e y r => free_immut_in x e || (negb (String.eqb x y) && free_immut_in x r)
     end.
@@ -118,7 +120,7 @@ Section Examples.
                         (EAtom (ANil None)))
                      (EAtom (ANil None)))).
     reflexivity. Abort.
-  Compute to_join_head ex2.
+  (* Compute to_join_head ex2. *)
 
   Definition filter_pushdown_head (e : expr) :=
     match e with
@@ -152,8 +154,8 @@ Section Examples.
                (EAtom (ANil None)))
             (EAtom (ANil None)))).
     reflexivity. Abort.
-  Compute (fold_expr to_join_head ex3).
-  Compute (fold_expr filter_pushdown_head (fold_expr to_join_head ex3)).
+  (* Compute (fold_expr to_join_head ex3).
+  Compute (fold_expr filter_pushdown_head (fold_expr to_join_head ex3)). *)
 
   Section WithMap.
     Context {tenv: map.map string type} {tenv_ok: map.ok tenv}.
@@ -167,18 +169,6 @@ Section Examples.
           let E := fresh "E" in
           destruct x eqn:E
       end.
-
-    Local Ltac apply_type_sound :=
-    lazymatch goal with
-    | H : type_of _ _ ?e (TList ?t), E : interp_expr _ _ ?e = _ |- type_of_value _ ?t => eapply type_sound in H; eauto;
-                                                                                             rewrite E in H; inversion H; subst
-    | H : type_of _ _ ?e ?t |- type_of_value (interp_expr _ _ ?e) ?t => eapply type_sound in H; eauto
-    end.
-
-    Local Ltac apply_Forall_In_vlist :=
-        lazymatch goal with
-        | H : Forall (fun v => type_of_value v ?t) _ |- _ => eapply List.Forall_In in H; eauto
-        end.
 
     Lemma In_flat_map_ext : forall A B l (f : A -> list B) g,
         (forall a, In a l -> f a = g a) ->
@@ -216,18 +206,21 @@ Section Examples.
     Qed.
 
     Definition preserve_ty (f : expr -> expr) :=
-      forall Gstore Genv e t, type_of Gstore Genv e t -> type_of Gstore Genv (f e) t.
+      forall Gstore Genv e t,
+        tenv_wf Gstore -> tenv_wf Genv ->
+        type_of Gstore Genv e t -> type_of Gstore Genv (f e) t.
 
     Definition preserve_sem f :=
       forall Gstore Genv e t store env,
+        tenv_wf Gstore -> tenv_wf Genv ->
         type_of Gstore Genv e t ->
-        well_formed_locals Gstore store ->
-        well_formed_locals Genv env ->
+        locals_wf Gstore store ->
+        locals_wf Genv env ->
         interp_expr store env e = interp_expr store env (f e).
 
     Lemma to_filter_head_preserve_ty : preserve_ty to_filter_head.
     Proof.
-      unfold preserve_ty. intros.
+      unfold preserve_ty. intros Gstore Genv e t H_Gstore H_Genv H.
       destruct e; auto. destruct e2; auto. destruct e2_2; auto.
       destruct o; auto. destruct e2_2_1; auto. destruct e2_2_2; auto.
       destruct a, e2_3; auto. destruct a; auto.
@@ -235,13 +228,13 @@ Section Examples.
       rewrite eqb_eq in E; subst.
       inversion H; subst. inversion H5; subst. inversion H8; subst.
       inversion H7; subst. inversion H9; inversion H11; subst. rewrite map.get_put_same in *.
-      injection H13 as H13; subst.
+      injection H14 as H14; subst.
       constructor; auto.
     Qed.
 
     Lemma to_filter_head_preserve_sem : preserve_sem to_filter_head.
     Proof.
-      unfold preserve_sem. intros Gstore Genv e t store env H H_str H_env.
+      unfold preserve_sem. intros Gstore Genv e t store env H_Gstore H_Genv H H_str H_env.
       destruct e; auto. destruct e2; auto. destruct e2_2; auto.
       destruct o; auto. destruct e2_2_1; auto. destruct e2_2_2; auto. destruct a, e2_3; auto.
       destruct a; auto. simpl. destruct (x =? x0) eqn:E; auto. simpl.
@@ -288,14 +281,21 @@ Section Examples.
         subst. simpl in H; rewrite Bool.orb_false_iff in *. constructor; inversion H0; subst.
         + apply H3; destruct a; intuition.
         + fold (map snd l) (map snd tl). apply IHl; intuition.
-      - inversion H1; subst. constructor. clear H1. induction l; auto.
+      - inversion H1; subst. constructor; auto. clear H1. induction l; auto.
         simpl in H; rewrite Bool.orb_false_iff in *. constructor.
-        + inversion H3. inversion H0; subst. split; apply H8;
+        + inversion H5. inversion H0; subst. split; apply H10;
             destruct a; rewrite Bool.orb_false_iff in *; intuition.
-        + inversion H0; inversion H3. apply IHl; intuition.
+        + inversion H5; inversion H0. apply IHl; intuition.
       - inversion H0; subst. econstructor.
         + apply IHe1; eauto; intuition.
         + apply IHe2; eauto; intuition.
+      - inversion H0; subst. econstructor.
+        + apply IHe1; eauto; intuition.
+        + apply IHe2; eauto; intuition.
+        + destruct (x =? x0) eqn:Ex.
+          * rewrite eqb_eq in *; subst. rewrite Properties.map.put_put_same in *; auto.
+          * apply IHe3; intuition.
+            rewrite eqb_neq in *. rewrite Properties.map.put_put_diff; auto.
       - inversion H0; subst. constructor.
         + apply IHe1; auto; intuition.
         + destruct (x =? x0) eqn:Ex.
@@ -369,6 +369,11 @@ Section Examples.
       - rewrite <- IHe1, <- IHe2, <- IHe3; auto; intuition.
       - rewrite <- IHe1, <- IHe2; auto; intuition.
       - rewrite <- IHe1, <- IHe2; auto; intuition.
+      - rewrite <- IHe1, <- IHe2; auto; intuition. repeat destruct_one_match; auto.
+        destruct (x0 =? x) eqn:Ex.
+          * rewrite eqb_eq in *; subst.
+            rewrite Properties.map.put_put_same. auto.
+          * rewrite eqb_neq in *. rewrite Properties.map.put_put_diff with (k1 := x0); intuition.
       - rewrite <- IHe1; intuition. destruct_one_match; auto.
         f_equal. clear E. induction l; auto. simpl.
          destruct (x0 =? x) eqn:E'.
@@ -416,7 +421,7 @@ Section Examples.
 
     Lemma to_join_head_preserve_ty : preserve_ty to_join_head.
     Proof.
-      unfold preserve_ty. intros.
+      unfold preserve_ty. intros Gstore Genv e t H_Gstore H_Genv H.
       destruct e; auto. destruct e2; auto. destruct e2_2; auto.
       destruct e2_2_2; auto. destruct o; auto. destruct e2_2_2_2; auto.
       destruct a; auto. destruct e2_2_3; auto. destruct a; auto.
@@ -429,19 +434,22 @@ Section Examples.
     Qed.
 
     Lemma to_join_head_preserve_sem' : forall (store env: locals) (Gstore Genv: tenv) (tbl1 tbl2 p r : expr) (x y : string) (t1 t2 t3 : type) (t t' : option type),
+        tenv_wf Gstore -> tenv_wf Genv ->
         type_of Gstore Genv tbl1 (TList t1) ->
         type_of Gstore (map.put Genv x t1) tbl2 (TList t2) ->
         free_immut_in x tbl2 = false ->
         type_of Gstore (map.put (map.put Genv x t1) y t2) p TBool ->
-        well_formed_locals Gstore store ->
-        well_formed_locals Genv env ->
+        locals_wf Gstore store ->
+        locals_wf Genv env ->
         interp_expr store env (EFlatmap tbl1 x
                        (EFlatmap tbl2 y
                           (EIf p (EBinop OCons r (EAtom (ANil t))) (EAtom (ANil t'))))) =
           interp_expr store env (EJoin tbl1 tbl2 x y p r).
     Proof.
-      intros store env Gstore Genv tbl1 tbl2 p r x y t1 t2 t3 t t' H_tbl1 H_tbl2 H_free H_p H_str H_env.
-      simpl. eapply type_sound in H_tbl1; eauto. inversion H_tbl1; subst.
+      intros store env Gstore Genv tbl1 tbl2 p r x y t1 t2 t3 t t' H_Gstore H_Genv H_tbl1 H_tbl2 H_free H_p H_str H_env.
+      simpl. apply type_of__type_wf in H_tbl1 as H_wf1; auto. apply type_of__type_wf in H_tbl2 as H_wf2; auto;
+        [| apply tenv_wf_step; inversion H_wf1]; auto.
+      eapply type_sound in H_tbl1; eauto. inversion H_tbl1; subst.
       f_equal. apply not_free_immut_put_ty in H_tbl2 as H_tbl2'; auto.
       eapply type_sound in H_tbl2'; eauto. inversion H_tbl2'; subst.
       f_equal. apply flat_map_eq. rewrite Forall_forall. intros v H_v.
@@ -453,25 +461,31 @@ Section Examples.
         eapply type_sound in H_p; eauto.
         + inversion H_p; subst. rewrite <- H2. destruct b; simpl; [f_equal |];
             inversion H3; inversion H5; apply IHl1; auto.
-        + rewrite Forall_forall in *; repeat apply well_formed_locals_step; intuition.
-      - rewrite Forall_forall in *; repeat apply well_formed_locals_step; intuition.
+        + rewrite Forall_forall in *; repeat apply locals_wf_step;
+            repeat apply tenv_wf_step; intuition;
+            inversion H_wf1; inversion H_wf2; auto.
+        + repeat apply locals_wf_step; auto.
+          * eapply List.Forall_In in H1; eauto.
+          * inversion H3; auto.
+      - apply tenv_wf_step; auto. inversion H_wf1; auto.
+      - rewrite Forall_forall in *; repeat apply locals_wf_step; intuition.
     Qed.
 
     Lemma to_join_head_preserve_sem : preserve_sem to_join_head.
     Proof.
-      unfold preserve_sem. intros.
+      unfold preserve_sem. intros Gstore Genv e t store env H_Gstore H_Genv H H_str H_env.
       destruct e; auto. destruct e2; auto. destruct e2_2; auto.
       destruct e2_2_2; auto. destruct o; auto. destruct e2_2_2_2; auto.
       destruct a; auto. destruct e2_2_3; auto. destruct a; auto.
       unfold to_join_head. destruct ((x =? x0) || free_immut_in x e2_1)%bool eqn:E; auto.
-      inversion H; subst. inversion H7; subst. inversion H9; subst. inversion H11; subst.
+      inversion H; subst. inversion H5; subst. inversion H7; subst. inversion H9; subst.
       rewrite Bool.orb_false_iff in *.
-      eapply to_join_head_preserve_sem'; eauto; intuition.
+      eapply to_join_head_preserve_sem' with (Gstore := Gstore); eauto; intuition.
     Qed.
 
     Lemma filter_pushdown_head_preserve_ty : preserve_ty filter_pushdown_head.
     Proof.
-      unfold preserve_ty. intros.
+      unfold preserve_ty. intros Gstore Genv e t H_Gstore H_Genv H.
       destruct e; auto. destruct e3; auto. destruct o; auto.
       simpl. destruct_one_match; auto.
       inversion H; subst. inversion H9; subst. inversion H3; subst.
@@ -488,27 +502,27 @@ Section Examples.
 
     Lemma filter_pushdown_head_preserve_sem : preserve_sem filter_pushdown_head.
     Proof.
-      unfold preserve_sem. intros.
+      unfold preserve_sem. intros Gstore Genv e t store env H_Gstore H_Genv H H_str H_env.
       destruct e; auto. destruct e3; auto. destruct o; auto.
       unfold filter_pushdown_head. destruct (free_immut_in y e3_1) eqn:E; auto.
 
       simpl. destruct (interp_expr store env e1) eqn:E1; auto.
       destruct (interp_expr store env e2) eqn:E2; auto. f_equal.
       inversion H; subst.
-      eapply type_sound in H9, H10; eauto. rewrite E1 in H9. rewrite E2 in H10.
-      inversion H9; inversion H10; subst.
+      eapply type_sound in H7, H8; eauto. rewrite E1 in H7. rewrite E2 in H8.
+      inversion H7; inversion H8; subst.
       rewrite flat_map_filter. apply In_flat_map_ext; intros.
       destruct (interp_expr store (map.put env x a) e3_1) eqn:E3_1;
-        try (clear E2 H10; induction l0; auto; simpl;
+        try (clear E2 H8; induction l0; auto; simpl;
              eapply not_free_immut_put_sem in E; rewrite <- E; rewrite E3_1; simpl;
-             apply IHl0; inversion H7; intuition).
+             apply IHl0; inversion H5; intuition).
       destruct b.
-      - clear E2 H10; induction l0; inversion H7; auto; simpl.
+      - clear E2 H8; induction l0; inversion H5; auto; simpl.
         eapply not_free_immut_put_sem in E; rewrite <- E; rewrite E3_1; simpl.
         destruct (interp_expr store (map.put (map.put env x a) y a0) e3_2) eqn:E3_2; simpl;
           try (apply IHl0; intuition).
         destruct b; simpl; [f_equal |]; apply IHl0; intuition.
-      - clear E2 H10; induction l0; inversion H7; auto; simpl.
+      - clear E2 H8; induction l0; inversion H5; auto; simpl.
         eapply not_free_immut_put_sem in E; rewrite <- E; rewrite E3_1; simpl.
         destruct (interp_expr store (map.put (map.put env x a) y a0) e3_2) eqn:E3_2; simpl;
           apply IHl0; intuition.
@@ -516,7 +530,9 @@ Section Examples.
 
     Local Ltac apply_fold_expr_IH' e :=
       lazymatch goal with
-      | IH : context [interp_expr _ _ e = interp_expr _ _ (fold_expr _ e)] |- _ => erewrite <- IH; clear IH; eauto
+      | H : type_of ?Gstore' _ _ _,
+          IH : context [interp_expr _ _ e = interp_expr _ _ (fold_expr _ e)] |- _ =>
+          erewrite <- IH with (Gstore := Gstore'); clear IH; eauto
       end.
 
     Local Ltac apply_fold_expr_IH :=
@@ -529,25 +545,64 @@ Section Examples.
       | H : type_of _ _ _ _ |- _ => inversion H; subst
       end.
 
+  Local Ltac invert_type_wf :=
+    lazymatch goal with
+    | H: type_wf (TList ?t) |- type_wf ?t => inversion H; clear H; subst
+    | H: type_wf (TOption ?t) |- type_wf ?t => inversion H; clear H; subst
+    | H: type_wf (TDict ?t _) |- type_wf ?t => inversion H; clear H; subst
+    | H: type_wf (TDict _ ?t) |- type_wf ?t => inversion H; clear H; subst
+    | H: type_wf (TRecord ?tl) |- Forall type_wf (List.map snd ?tl) => inversion H; clear H; subst
+    end.
+
+    Local Ltac apply_type_of__type_wf :=
+      lazymatch goal with
+      | H: type_of _ _ _ ?t |- type_wf ?t =>
+          let H' := fresh "H'" in
+          apply type_of__type_wf in H as H'
+      | H: type_of _ _ _ (TList ?t) |- type_wf ?t =>
+          let H' := fresh "H'" in
+          apply type_of__type_wf in H as H'
+      | H:  type_of _ _ _ (TOption ?t) |- type_wf ?t =>
+          let H' := fresh "H'" in
+          apply type_of__type_wf in H as H'
+      | H:  type_of _ _ _ (TDict ?t _) |- type_wf ?t =>
+          let H' := fresh "H'" in
+          apply type_of__type_wf in H as H'
+      | H:  type_of _ _ _ (TDict _ ?t) |- type_wf ?t =>
+          let H' := fresh "H'" in
+          apply type_of__type_wf in H as H'
+      | H:  type_of _ _ _ (TRecord ?tl) |- context[?tl] =>
+          let H' := fresh "H'" in
+          apply type_of__type_wf in H as H'
+      end.
+
     Theorem fold_expr_preserve_ty : forall f, preserve_ty f -> preserve_ty (fold_expr f).
     Proof.
       unfold preserve_ty. intros f H Gstore Genv e.
       revert Gstore Genv. induction e using expr_IH;
         intros; simpl; auto;
-        apply H; invert_type_of; subst; econstructor; eauto.
+        apply H; invert_type_of; subst; try econstructor; eauto.
+      all: try apply IHe2; auto; repeat apply tenv_wf_step; auto; try apply_type_of__type_wf; auto;
+        try invert_type_wf; auto.
+      - apply IHe3; auto; repeat apply tenv_wf_step; auto;
+        apply type_of__type_wf in H9, H10; try invert_type_wf; auto.
       - rewrite fst_map_fst; auto.
-      - clear H1 H5 H6 H7. generalize dependent tl.
+      - clear H3 H7 H8 H9. generalize dependent tl.
         induction l; intros; destruct tl; try discriminate.
         + constructor.
         + simpl. constructor.
-          * inversion H0; subst. inversion H4; subst. apply H5 in H8.
+          * inversion H0; subst. inversion H6; subst. apply H7 in H10; auto.
             destruct a; simpl in *. auto.
-          * simpl in *; inversion H0; inversion H3; inversion H4; apply IHl; auto.
-      - rewrite fst_map_fst; auto.
+          * simpl in *; inversion H0; inversion H5; inversion H6; apply IHl; auto.
       - induction l; auto. constructor.
-        + destruct a; inversion H0; inversion H3; intuition.
-        + inversion H0; inversion H3; apply IHl; auto.
-          inversion H1; subst. constructor. auto.
+        + destruct a. inversion H0; inversion H7; intuition.
+        + inversion H0; inversion H7; apply IHl; auto.
+          inversion H3; subst. constructor; auto.
+      - apply IHe3; auto. apply tenv_wf_step; auto. apply_type_of__type_wf; try invert_type_wf; auto.
+      - apply IHe3; auto. repeat apply tenv_wf_step; auto;
+          apply_type_of__type_wf; try invert_type_wf; auto.
+      - apply IHe4; auto. repeat apply tenv_wf_step; auto;
+          apply_type_of__type_wf; try invert_type_wf; auto.
     Qed.
 
     Lemma In_map_snd : forall A B (a : A) (b : B) l, In (a, b) l -> In b (List.map snd l).
@@ -564,107 +619,158 @@ Section Examples.
       erewrite IHl; eauto. intuition.
     Qed.
 
+    Local Ltac apply_type_sound :=
+    lazymatch goal with
+    | H : type_of _ _ ?e (TList ?t), E : interp_expr _ _ ?e = _ |- type_of_value _ ?t =>
+        eapply type_sound in H; eauto; rewrite E in H; inversion H; subst
+    | H : type_of _ _ ?e (TOption ?t), E : interp_expr _ _ ?e = _ |- type_of_value _ ?t =>
+        eapply type_sound in H; eauto; rewrite E in H; inversion H; subst
+    | H : type_of _ _ ?e ?t |- type_of_value (interp_expr _ _ ?e) ?t =>
+        eapply type_sound in H; eauto
+    | H : type_of _ _ ?e ?t,
+        H1 : In ?v ?l,
+          E : interp_expr _ _ ?e = Value.VList ?l
+      |- type_of_value ?v ?t =>
+        eapply type_sound in H; eauto; rewrite E in H; inversion H; subst
+    end.
+
     Theorem fold_expr_preserve_sem : forall f, preserve_ty f -> preserve_sem f -> preserve_sem (fold_expr f).
     Proof.
       unfold preserve_sem. intros f H_ty H_sem Gstore Genv e; revert Gstore Genv.
       induction e using expr_IH;
         intros; simpl;
-        try now (erewrite <- H_sem; eauto).
-      - invert_type_of. erewrite <- H_sem; simpl; repeat apply_fold_expr_IH; eauto.
+        try now (erewrite <- H_sem with (Gstore := Gstore); eauto).
+      - invert_type_of. erewrite <- H_sem with (Gstore := Gstore); simpl; repeat apply_fold_expr_IH; eauto.
         econstructor; eauto; apply fold_expr_preserve_ty; auto.
-      - invert_type_of. subst. erewrite <- H_sem; simpl; repeat apply_fold_expr_IH; eauto.
+      - invert_type_of. subst. erewrite <- H_sem with (Gstore := Gstore); simpl; repeat apply_fold_expr_IH; eauto.
         econstructor; eauto; apply fold_expr_preserve_ty; eauto.
-      - invert_type_of. erewrite <- H_sem; simpl; repeat apply_fold_expr_IH; eauto.
+      - invert_type_of. erewrite <- H_sem with (Gstore := Gstore); simpl; repeat apply_fold_expr_IH; eauto.
         econstructor; apply fold_expr_preserve_ty; eauto.
-      - invert_type_of. erewrite <- H_sem; simpl; repeat apply_fold_expr_IH; eauto;
-          try (econstructor; apply fold_expr_preserve_ty; eauto).
-        apply well_formed_locals_step; auto. eapply type_sound; eauto.
-      - invert_type_of. erewrite <- H_sem; simpl; repeat apply_fold_expr_IH; eauto;
-          try (econstructor; apply fold_expr_preserve_ty; eauto).
-        destruct_one_match; auto.
-        f_equal. apply In_flat_map_ext; intros. repeat apply_fold_expr_IH; eauto.
-        apply well_formed_locals_step; auto. apply_type_sound. apply_Forall_In_vlist.
-      - invert_type_of. erewrite <- H_sem; simpl; repeat apply_fold_expr_IH; eauto;
-          try (econstructor; apply fold_expr_preserve_ty; eauto).
-        destruct_one_match; auto. apply_fold_expr_IH' e2; eauto.
-        apply In_fold_right_ext with (P := fun v => type_of_value v t); intros.
-        + apply_type_sound.
-        + apply_fold_expr_IH; eauto; intuition.
-          * apply_type_sound. repeat apply well_formed_locals_step; auto.
-            apply_type_sound; apply_Forall_In_vlist.
-          * repeat apply well_formed_locals_step; auto. apply_type_sound; apply_Forall_In_vlist.
-      - invert_type_of. erewrite <- H_sem; simpl; eauto.
+      - invert_type_of. erewrite <- H_sem with (Gstore := Gstore); simpl; eauto.
+        + erewrite <- IHe2. 4: eassumption.
+          all: auto; repeat apply_fold_expr_IH;
+            try apply locals_wf_step; try apply tenv_wf_step; try eapply type_sound; eauto.
+          apply_type_of__type_wf; auto.
+        + econstructor; apply fold_expr_preserve_ty; eauto. apply tenv_wf_step; try apply_type_of__type_wf; auto.
+      - invert_type_of. erewrite <- H_sem with (Gstore := Gstore); simpl; repeat apply_fold_expr_IH; eauto.
+        + destruct_one_match; auto. f_equal. apply In_flat_map_ext; intros.
+          erewrite <- IHe2. 4: eassumption.
+          all: auto; try apply locals_wf_step; try apply tenv_wf_step; try apply_type_of__type_wf; try invert_type_wf; auto.
+          apply_type_sound. rewrite Forall_forall in *; auto.
+        + econstructor; apply fold_expr_preserve_ty; eauto.
+          apply tenv_wf_step; try apply_type_of__type_wf; try invert_type_wf; auto.
+      - invert_type_of. erewrite <- H_sem with (Gstore := Gstore); simpl; repeat apply_fold_expr_IH; eauto.
+        + destruct_one_match; auto. apply_fold_expr_IH' e2; eauto.
+          apply In_fold_right_ext with (P := fun v => type_of_value v t); intros; try apply_type_sound.
+          erewrite <- IHe3. 4: eassumption. all: intuition.
+          * apply_type_sound; repeat apply locals_wf_step; repeat apply tenv_wf_step; auto.
+            -- apply_type_of__type_wf; auto. invert_type_wf; auto.
+            -- apply type_of__type_wf in H11; auto.
+            -- apply_type_sound. rewrite Forall_forall in *; auto.
+          * repeat apply tenv_wf_step; auto.
+            -- apply_type_of__type_wf; auto. invert_type_wf; auto.
+            -- apply type_of__type_wf in H11; auto.
+          * repeat apply locals_wf_step; auto.
+            apply_type_sound. rewrite Forall_forall in *; auto.
+        + try (econstructor; apply fold_expr_preserve_ty; eauto).
+          repeat apply tenv_wf_step; auto.
+            -- apply_type_of__type_wf; auto. invert_type_wf; auto.
+            -- apply type_of__type_wf in H11; auto.
+      - invert_type_of. erewrite <- H_sem with (Gstore := Gstore); simpl; eauto.
         + do 2 f_equal. rewrite map_map; apply map_ext_Forall; rewrite Forall_forall.
           intros x H_in; destruct x. pose proof In_map_snd.
           match goal with
-          | H : Forall2 _ _ _ |- _ => eapply Forall2_In_Permuted in H; eauto; do 3 destruct H5
+          | H : Forall2 _ _ _ |- _ => eapply Forall2_In_Permuted in H; eauto; do 3 destruct H
           end.
           intuition; f_equal.
-          rewrite Forall_forall in *. eapply H in H_in; simpl in *; eauto.
+          rewrite Forall_forall in *. eapply H with (Gstore := Gstore) in H_in; simpl in *; eauto.
         + econstructor; eauto; try (rewrite fst_map_fst; auto).
           apply fold_expr_preserve_ty in H_ty.
-          clear H0 H6 H7. generalize dependent tl. induction l; destruct tl; try discriminate; intuition.
-          simpl. inversion H5; subst. constructor.
-          * destruct a. simpl. apply H_ty. auto.
-          * inversion H4; inversion H; apply IHl; auto.
-      - invert_type_of. erewrite <- H_sem; simpl; eauto; try apply_fold_expr_IH r.
+          clear H2 H8 H9. generalize dependent tl. induction l; destruct tl; try discriminate; intuition.
+          simpl. inversion H7; subst. constructor.
+          * destruct a. simpl. apply H_ty; auto.
+          * inversion H6; inversion H; apply IHl; auto.
+      - invert_type_of. erewrite <- H_sem with (Gstore := Gstore); simpl; eauto; try apply_fold_expr_IH r.
         econstructor; eauto. apply fold_expr_preserve_ty; auto.
-      - invert_type_of. erewrite <- H_sem; simpl; eauto.
+      - invert_type_of. erewrite <- H_sem with (Gstore := Gstore); simpl; eauto.
         + do 2 f_equal. rewrite map_map; apply map_ext_Forall; rewrite Forall_forall.
           intros x H_in; destruct x eqn:E.
           apply Forall_and_inv in H. intuition. rewrite Forall_forall in *.
-          f_equal; [ pose proof (H3 x) | pose proof (H5 x) ]; subst; simpl in *; eapply H; eauto;
-            apply H4 in H_in; simpl in *; apply H_in.
-        + constructor. rewrite Forall_forall. intros p H_in.
-          apply in_map_iff in H_in as [[k v] [H_p_p0 H_in]]; subst.
-          rewrite Forall_forall in *. apply H4 in H_in as [H4L H4R].
-          eapply fold_expr_preserve_ty in H4L, H4R; eauto.
-      - invert_type_of. erewrite <- H_sem; simpl; eauto; try apply_fold_expr_IH.
+          f_equal; [ pose proof (H5 x) | pose proof (H9 x) ]; subst; simpl in *; eapply H with (Gstore := Gstore); eauto;
+            apply H8 in H_in; simpl in *; apply H_in.
+        + constructor.
+          3: rewrite Forall_forall; intros p H_in;
+          apply in_map_iff in H_in as [[k v] [H_p_p0 H_in]]; subst;
+          rewrite Forall_forall in *; apply H8 in H_in as [HL HR];
+          eapply fold_expr_preserve_ty in HL, HR; eauto.
+          all: auto.
+      - invert_type_of. erewrite <- H_sem with (Gstore := Gstore); simpl; eauto; try apply_fold_expr_IH.
         + destruct_one_match; auto. do 2 f_equal; apply_fold_expr_IH.
         + constructor; apply fold_expr_preserve_ty; eauto.
-      - invert_type_of. erewrite <- H_sem; simpl; eauto; try apply_fold_expr_IH.
+      - invert_type_of. erewrite <- H_sem with (Gstore := Gstore); simpl; eauto; try apply_fold_expr_IH.
         + destruct_one_match; auto. do 2 f_equal; apply_fold_expr_IH.
         + constructor; apply fold_expr_preserve_ty; eauto.
-      - invert_type_of. erewrite <- H_sem; simpl; eauto; try apply_fold_expr_IH.
+      - invert_type_of. erewrite <- H_sem with (Gstore := Gstore); simpl; eauto; try apply_fold_expr_IH.
         + destruct_one_match; auto. do 2 f_equal; apply_fold_expr_IH.
         + econstructor; apply fold_expr_preserve_ty; eauto.
-      - invert_type_of. erewrite <- H_sem; simpl; eauto; try apply_fold_expr_IH.
+      - invert_type_of. erewrite <- H_sem with (Gstore := Gstore); simpl; eauto; try apply_fold_expr_IH.
+        + repeat destruct_one_match; auto.
+          2: apply_fold_expr_IH; auto.
+          erewrite <- IHe3. 4: eassumption.
+          all: auto; try apply locals_wf_step; try apply tenv_wf_step; auto.
+          * apply_type_of__type_wf; auto; invert_type_wf; auto.
+          * apply_type_sound; auto.
+        + econstructor; apply fold_expr_preserve_ty; eauto. apply tenv_wf_step; auto.
+          apply_type_of__type_wf; auto; invert_type_wf; auto.
+      - invert_type_of. erewrite <- H_sem with (Gstore := Gstore); simpl; eauto; try apply_fold_expr_IH.
         + destruct_one_match; auto. f_equal.
-          apply In_filter_ext. intros x0 H_in. apply_fold_expr_IH.
-          apply well_formed_locals_step; auto. apply_type_sound; apply_Forall_In_vlist.
-        + constructor; apply fold_expr_preserve_ty; eauto.
-      - invert_type_of. erewrite <- H_sem; simpl; eauto; try apply_fold_expr_IH.
+          apply In_filter_ext. intros x0 H_in.
+          erewrite <- IHe2. 4: eassumption.
+          all: try apply locals_wf_step; try apply tenv_wf_step; auto.
+          * apply_type_of__type_wf; auto; invert_type_wf; auto.
+          * apply_type_sound. rewrite Forall_forall in *; auto.
+        + constructor; apply fold_expr_preserve_ty; eauto. apply tenv_wf_step; auto.
+          apply_type_of__type_wf; auto; invert_type_wf; auto.
+      - invert_type_of. erewrite <- H_sem with (Gstore := Gstore); simpl; eauto; try apply_fold_expr_IH.
         + destruct_one_match; auto. apply_fold_expr_IH.
           destruct_one_match; auto. f_equal.
           apply In_flat_map_ext. intros a H_in_a. erewrite In_filter_ext; try apply map_ext_Forall.
           * rewrite Forall_forall. intros x0 H_in_x0. rewrite filter_In in H_in_x0; intuition.
-            apply_fold_expr_IH. repeat apply well_formed_locals_step; auto;
-              apply_type_sound; apply_Forall_In_vlist.
-          * intros x0 H_in_x0. simpl. apply_fold_expr_IH.
-            repeat apply well_formed_locals_step; auto;
-              apply_type_sound; apply_Forall_In_vlist.
-        + econstructor; apply fold_expr_preserve_ty; eauto.
-      - invert_type_of. erewrite <- H_sem; simpl; eauto; try apply_fold_expr_IH.
+            erewrite <- IHe4. 4: eassumption.
+            all: repeat apply locals_wf_step; repeat apply tenv_wf_step; auto.
+            1,2: apply_type_of__type_wf; auto; invert_type_wf; auto.
+            1,2: apply_type_sound; rewrite Forall_forall in *; auto.
+          * intros x0 H_in_x0. simpl. erewrite <- IHe3. 4: eassumption.
+            all: repeat apply locals_wf_step; repeat apply tenv_wf_step; auto.
+            1,2: apply_type_of__type_wf; auto; invert_type_wf; auto.
+            1,2: apply_type_sound; rewrite Forall_forall in *; auto.
+        + econstructor; apply fold_expr_preserve_ty; eauto; repeat apply tenv_wf_step; auto;
+          apply_type_of__type_wf; auto; invert_type_wf; auto.
+      - invert_type_of. erewrite <- H_sem with (Gstore := Gstore); simpl; eauto; try apply_fold_expr_IH.
         + destruct_one_match; auto. f_equal. apply map_ext_Forall; rewrite Forall_forall.
-          intros x0 H_in. apply_fold_expr_IH. apply well_formed_locals_step; auto.
-          apply_type_sound; apply_Forall_In_vlist.
-        + econstructor; apply fold_expr_preserve_ty; eauto.
+          intros x0 H_in. erewrite <- IHe2. 4: eassumption.
+          all: try apply locals_wf_step; try apply tenv_wf_step; auto.
+          * apply_type_of__type_wf; auto; invert_type_wf; auto.
+          * apply_type_sound; rewrite Forall_forall in *; auto.
+        + econstructor; apply fold_expr_preserve_ty; eauto. repeat apply tenv_wf_step; auto.
+          apply_type_of__type_wf; auto; invert_type_wf; auto.
     Qed.
 
-    Compute ex3.
+    (* Compute ex3. *)
     Definition ex3_op := fold_expr filter_pushdown_head (fold_expr to_join_head ex3).
-    Compute ex3_op.
+    (* Compute ex3_op. *)
     Lemma ex3_op_equiv_ex3 : forall Gstore Genv t store env,
+        tenv_wf Gstore -> tenv_wf Genv ->
         type_of Gstore Genv ex3 t ->
-        well_formed_locals Gstore store ->
-        well_formed_locals Genv env ->
+        locals_wf Gstore store ->
+        locals_wf Genv env ->
         type_of Gstore Genv ex3_op t /\ interp_expr store env ex3 = interp_expr store env ex3_op.
     Proof.
       intros; unfold ex3_op. split.
-      - apply fold_expr_preserve_ty; [apply filter_pushdown_head_preserve_ty |].
-        apply fold_expr_preserve_ty; [apply to_join_head_preserve_ty | auto].
-      - erewrite fold_expr_preserve_sem; eauto.
-        + erewrite fold_expr_preserve_sem; eauto.
+      - apply fold_expr_preserve_ty; auto; [apply filter_pushdown_head_preserve_ty |].
+        apply fold_expr_preserve_ty; auto; apply to_join_head_preserve_ty.
+      - erewrite fold_expr_preserve_sem with (Gstore := Gstore); eauto.
+        + erewrite fold_expr_preserve_sem with (Gstore := Gstore); eauto.
           * exact filter_pushdown_head_preserve_ty.
           * exact filter_pushdown_head_preserve_sem.
           * apply fold_expr_preserve_ty; eauto. exact to_join_head_preserve_ty.
