fiat2/src/fiat2/TypeSound.v
@@ -11,7 +11,7 @@ Section WithWord.
 
   Section WithMap.
     Context {tenv: map.map string type} {tenv_ok: map.ok tenv}.
-    Local Notation value := (value (word := word)).
+    Local Notation value := (Value.value (word := word)).
     Context {locals: map.map string value} {locals_ok: map.ok locals}.
 
     Local Coercion is_true : bool >-> Sortclass.
@@ -25,27 +25,28 @@ Section WithWord.
     | TyVOptionSome v t : type_of_value v t ->
                           type_of_value (VOption (Some v)) (TOption t)
     | TyVList l t : Forall (fun v => type_of_value v t) l -> type_of_value (VList l) (TList t)
-    | TyVRecord l tl : NoDup (List.map fst l) -> StronglySorted record_entry_leb l ->
+    | TyVRecord l tl : NoDup (List.map fst tl) -> StronglySorted record_entry_leb tl ->
                        Forall2 (fun p tp => fst p = fst tp /\ type_of_value (snd p) (snd tp)) l tl ->
                        type_of_value (VRecord l) (TRecord tl)
-    | TyVDict l tk tv : Forall (fun p => type_of_value (fst p) tk /\ type_of_value (snd p) tv) l ->
+    | TyVDict l tk tv : type_wf tk -> type_wf tv ->
+                        Forall (fun p => type_of_value (fst p) tk /\ type_of_value (snd p) tv) l ->
                         type_of_value (VDict l) (TDict tk tv)
     | TyVUnit : type_of_value VUnit TUnit.
 
-  Definition well_formed_locals (G : tenv) (E : locals) :=
+  Definition locals_wf (G : tenv) (E : locals) :=
     forall x t, map.get G x = Some t ->
                 match map.get E x with
                 | Some v => type_of_value v t
                 | _ => False
                 end.
 
-  Lemma well_formed_locals_step : forall G E,
-      well_formed_locals G E ->
+  Lemma locals_wf_step : forall G E,
+      locals_wf G E ->
       forall x t v,
         type_of_value v t ->
-        well_formed_locals (map.put G x t) (map.put E x v).
+        locals_wf (map.put G x t) (map.put E x v).
   Proof.
-    unfold well_formed_locals; intros.
+    unfold locals_wf; intros.
     destruct (String.eqb x0 x) eqn:E_x.
     - rewrite String.eqb_eq in E_x. rewrite E_x in *.
       rewrite map.get_put_same. rewrite map.get_put_same in H1. congruence.
@@ -66,6 +67,15 @@ Section WithWord.
   Local Ltac destruct_compare_types :=
     unfold compare_types in *; destruct_match; constructor.
 
+  Local Ltac invert_type_wf :=
+    lazymatch goal with
+    | H: type_wf (TList ?t) |- type_wf ?t => inversion H; clear H; subst
+    | H: type_wf (TOption ?t) |- type_wf ?t => inversion H; clear H; subst
+    | H: type_wf (TDict ?t _) |- type_wf ?t => inversion H; clear H; subst
+    | H: type_wf (TDict _ ?t) |- type_wf ?t => inversion H; clear H; subst
+    | H: type_wf (TRecord ?tl) |- Forall type_wf (List.map snd ?tl) => inversion H; clear H; subst
+    end.
+
   Local Ltac invert_result :=
     lazymatch goal with
     | H: Success _ = Success _ |- _ => inversion H; clear H; intros; subst
@@ -78,174 +88,219 @@ Section WithWord.
 
   Lemma atom_typechecker_sound : forall a t a',
       (synthesize_atom a = Success (t, a') -> type_of_atom a t) /\
-        (analyze_atom t a = Success a' -> type_of_atom a t).
+        (analyze_atom t a = Success a' -> type_wf t -> type_of_atom a t).
   Proof.
-    destruct a; split; simpl; intro;
-      repeat (try destruct_compare_types; try destruct_match; try invert_result; try constructor).
+    destruct a; split; simpl; intro.
+    all: try (invert_result; constructor).
+    all: try destruct_compare_types.
+    1, 3: repeat destruct_match; invert_result; constructor; apply type_wf_comp_sound; auto.
+    1, 2: repeat destruct_match;
+    [ destruct_compare_types; invert_result; invert_type_wf; auto
+    | invert_result; constructor; invert_type_wf; auto ].
   Qed.
 
-  Local Ltac apply_typechecker_IH :=
-    match goal with
-    | IH: (forall _ _ _ _, (synthesize_expr _ _ ?e = _ -> _) /\ _),
-        H: synthesize_expr _ _ ?e = _ |- _ => eapply IH in H; eauto
-    | IH: (forall _ _ _ _, _ /\ (analyze_expr _ _ _ ?e = _ -> _)),
-        H: analyze_expr _ _ _ ?e = _ |- _ => eapply IH in H; eauto
-    end.
+  Lemma fst_map_fst : forall (A B C : Type) (l : list (A * B)) (f : A -> B -> C),
+      List.map fst (List.map (fun '(a, b) => (a, f a b)) l) = List.map fst l.
+  Proof.
+    induction l; auto.
+    intros. destruct a. simpl. f_equal. auto.
+  Qed.
 
-    Section __.
-    Lemma fst_map_fst : forall (A B C : Type) (l : list (A * B)) (f : A -> B -> C),
-        List.map fst (List.map (fun '(a, b) => (a, f a b)) l) = List.map fst l.
-    Proof.
-      induction l; auto.
-      intros. destruct a. simpl. f_equal. auto.
-    Qed.
-
-    Lemma inb_false_iff : forall s l, inb eqb l s = false <-> ~ In s l.
-    Proof.
-      induction l; simpl; intros.
-      - intuition.
-      - destruct (String.eqb a s) eqn:E; intuition.
-        + rewrite String.eqb_eq in E; intuition.
-        + rewrite String.eqb_neq in E; intuition.
-    Qed.
-
-    Lemma inb_true_iff : forall s l, inb eqb l s = true <-> In s l.
-    Proof.
-      induction l; simpl; intros.
-      - split; intuition.
-      - destruct (String.eqb a s) eqn:E; intuition.
-        + rewrite String.eqb_eq in E; intuition.
-        + rewrite String.eqb_neq in E; intuition.
-    Qed.
-
-    Lemma inclb_correct : forall l l', inclb String.eqb l l' = true -> incl l l'.
-    Proof.
-      induction l; simpl; intros.
-      - apply incl_nil_l.
-      - rewrite Bool.andb_true_iff in H. destruct H as [HL HR].
-        apply IHl in HR. rewrite inb_true_iff in HL.
-        unfold incl. intros. inversion H; subst; intuition.
-    Qed.
-
-    Lemma inclb_complete : forall l l', incl l l' -> inclb String.eqb l l' = true.
-    Proof.
-      intros l l' H. unfold inclb. rewrite forallb_forall; intros.
-      rewrite inb_true_iff. intuition.
-    Qed.
-
-    Lemma record_type_from'_sound : forall l tl el Gstore Genv,
-        Forall
+  Lemma record_type_from'_sound : forall l tl el (Gstore Genv : tenv),
+       Forall
+         (fun p : string * expr =>
+            forall (Gstore0 Genv0 : tenv) (t : type) (e' : expr),
+              tenv_wf Gstore0 ->
+              tenv_wf Genv0 ->
+              (synthesize_expr Gstore0 Genv0 (snd p) = Success (t, e') -> type_of Gstore0 Genv0 (snd p) t) /\
+                (analyze_expr Gstore0 Genv0 t (snd p) = Success e' -> type_wf t -> type_of Gstore0 Genv0 (snd p) t)) l ->
+       tenv_wf Gstore ->
+       tenv_wf Genv ->
+       record_type_from' (map (fun '(s, e') => (s, synthesize_expr Gstore Genv e')) l) = Success (tl, el) ->
+       map fst l = map fst tl /\ Forall2 (type_of Gstore Genv) (map snd l) (map snd tl) /\ NoDup (map fst l).
+  Proof.
+    induction l; intros.
+    - simpl in *. invert_result. intuition. apply NoDup_nil.
+    - simpl in *. repeat destruct_match. invert_result. destruct a. inversion E; subst; simpl.
+      inversion H; subst. apply (IHl _ _ _ _ H6) in E2; auto. intuition.
+      + f_equal. auto.
+      + constructor; auto. apply H5 in H4; auto.
+      + constructor; auto. apply inb_false_iff. erewrite <- fst_map_fst. apply E4.
+  Qed.
+(*
+  Lemma record_type_from'_sound : forall l tl el Gstore Genv,
+      Forall
         (fun p : string * expr =>
-         forall (Gstore Genv : tenv) (t : type) (e' : expr),
-         (synthesize_expr Gstore Genv (snd p) = Success (t, e') -> type_of Gstore Genv (snd p) t) /\
-         (analyze_expr Gstore Genv t (snd p) = Success e' -> type_of Gstore Genv (snd p) t)) l ->
-        record_type_from' (List.map (fun '(s, e') => (s, synthesize_expr Gstore Genv e')) l) = Success (tl, el) ->
-        List.map fst l = List.map fst tl /\ Forall2 (type_of Gstore Genv) (List.map snd l) (List.map snd tl) /\ NoDup (List.map fst l).
-    Proof.
-      induction l; intros.
-      - simpl in *. invert_result. intuition. apply NoDup_nil.
-      - simpl in *. repeat destruct_match. invert_result. destruct a. inversion E; subst; simpl.
-        inversion H; subst. apply (IHl _ _ _ _ H4)in E2 as [IHl1 [IHl2 IHl3]]. split; [| split].
-        + f_equal. auto.
-        + constructor; auto. apply H3 in H2. auto.
-        + constructor; auto. apply inb_false_iff. erewrite <- fst_map_fst. apply E4.
-    Qed.
+           forall (Gstore Genv : tenv) (t : type) (e' : expr),
+             (synthesize_expr Gstore Genv (snd p) = Success (t, e') -> type_of Gstore Genv (snd p) t) /\
+               (analyze_expr Gstore Genv t (snd p) = Success e' -> type_of Gstore Genv (snd p) t)) l ->
+      record_type_from' (List.map (fun '(s, e') => (s, synthesize_expr Gstore Genv e')) l) = Success (tl, el) ->
+      List.map fst l = List.map fst tl /\ Forall2 (type_of Gstore Genv) (List.map snd l) (List.map snd tl) /\ NoDup (List.map fst l).
+  Proof.
+    induction l; intros.
+    - simpl in *. invert_result. intuition. apply NoDup_nil.
+    - simpl in *. repeat destruct_match. invert_result. destruct a. inversion E; subst; simpl.
+      inversion H; subst. apply (IHl _ _ _ _ H4)in E2 as [IHl1 [IHl2 IHl3]]. split; [| split].
+      + f_equal. auto.
+      + constructor; auto. apply H3 in H2. auto.
+      + constructor; auto. apply inb_false_iff. erewrite <- fst_map_fst. apply E4.
+  Qed.
+ *)
 
-    Lemma record_from'_sound :
-      forall l tl' el Gstore Genv,
-        Forall
+  Lemma NoDup_In_get_attr_type : forall tl,  NoDup (List.map fst tl) -> forall s t, In (s, t) tl -> get_attr_type tl s = t.
+  Proof.
+    clear. induction tl; simpl; intros.
+    - intuition.
+    - destruct a. unfold get_attr_type; simpl. destruct (String.eqb s s0) eqn:E.
+      + intuition; try congruence. rewrite String.eqb_eq in E; inversion H; subst.
+        assert (In s0 (List.map fst tl)).
+        { clear H H3 H4 IHtl. induction tl; auto. destruct a; inversion H1; subst; simpl.
+          - left; congruence.
+          - right; auto. }
+        intuition.
+      + inversion H; subst. apply IHtl; auto. destruct H0; auto.
+        rewrite String.eqb_neq in E; inversion H0; congruence.
+  Qed.
+
+  Lemma Permutation_NoDup_In_get_attr_type : forall tl tl',
+      Permutation tl tl' -> NoDup (List.map fst tl') ->
+      forall s, In s (List.map fst tl') -> get_attr_type tl s = get_attr_type tl' s.
+  Proof.
+    intros.
+    assert (exists t, In (s, t) tl').
+    { clear H H0. induction tl'; simpl in *; intuition.
+      - exists (snd a). left; subst. apply surjective_pairing.
+      - destruct H0 as [t Ht]. firstorder. }
+    assert (NoDup (List.map fst tl)).
+    { apply Permutation_map with (f := fst) in H. apply Permutation_sym in H.
+      eapply Permutation_NoDup; eauto. }
+    destruct H2 as [t Ht]. repeat rewrite NoDup_In_get_attr_type with (t := t); auto.
+    apply Permutation_sym in H. eapply Permutation_in; eauto.
+  Qed.
+
+  Lemma In_fst : forall A B x (l : list (A * B)), In x (List.map fst l) -> exists p, In p l /\ fst p = x.
+  Proof.
+    induction l; simpl; intros; intuition.
+    - exists a. intuition.
+    - destruct H as [p H]; exists p; intuition.
+  Qed.
+
+  Lemma record_from'_sound :
+    forall l tl' el Gstore Genv,
+      Forall
         (fun p : string * expr =>
-         forall (Gstore Genv : tenv) (t : type) (e' : expr),
-         (synthesize_expr Gstore Genv (snd p) = Success (t, e') -> type_of Gstore Genv (snd p) t) /\
-         (analyze_expr Gstore Genv t (snd p) = Success e' -> type_of Gstore Genv (snd p) t)) l ->
-        record_from' (List.map (fun '(s, e) => (s, analyze_expr Gstore Genv (get_attr_type tl' s) e)) l) = Success el ->
-        let tl := List.map (fun '(s, _) => (s, get_attr_type tl' s)) l in
-        List.map fst l = List.map fst tl /\ Forall2 (type_of Gstore Genv) (List.map snd l) (List.map snd tl) /\ NoDup (List.map fst l).
-    Proof.
-      induction l; intros.
-      - simpl in *. invert_result. intuition. apply NoDup_nil.
-      - simpl in *. repeat destruct_match. destruct a. inversion H; inversion E; subst.
-        invert_result. simpl in *. intuition.
-        + f_equal. rewrite fst_map_fst. auto.
-        + constructor.
-          * eapply H3; eauto.
-          * eapply IHl; eauto.
-        + rewrite fst_map_fst in E2. apply inb_false_iff in E2. apply NoDup_cons; auto.
-          eapply IHl; eauto.
-    Qed.
+           forall (Gstore Genv : tenv) (t : type) (e' : expr),
+             tenv_wf Gstore ->
+             tenv_wf Genv ->
+             (synthesize_expr Gstore Genv (snd p) = Success (t, e') -> type_of Gstore Genv (snd p) t) /\
+               (analyze_expr Gstore Genv t (snd p) = Success e' -> type_wf t -> type_of Gstore Genv (snd p) t)) l ->
+      tenv_wf Gstore ->
+      tenv_wf Genv ->
+      type_wf (TRecord tl') ->
+      incl (List.map fst l) (List.map fst tl') ->
+      record_from' (List.map (fun '(s, e) => (s, analyze_expr Gstore Genv (get_attr_type tl' s) e)) l) = Success el ->
+      let tl := List.map (fun '(s, _) => (s, get_attr_type tl' s)) l in
+      List.map fst l = List.map fst tl /\ Forall2 (type_of Gstore Genv) (List.map snd l) (List.map snd tl) /\ NoDup (List.map fst l).
+  Proof.
+    induction l; intros tl' el Gstore Genv H H_Gstore H_Genv H_wf H_incl H_rec.
+    - simpl in *. invert_result. intuition. apply NoDup_nil.
+    - simpl in *. repeat destruct_match. destruct a. inversion H; inversion E; subst.
+      invert_result. simpl in *. intuition.
+      + f_equal. rewrite fst_map_fst. auto.
+      + constructor.
+        * eapply H2; eauto. inversion H_wf; subst.
+          unfold incl in *. simpl in *. assert (In s (List.map fst tl')). { intuition. }
+          apply In_fst in H0 as [p H0]. intuition. destruct p; simpl in *; subst.
+          eapply NoDup_In_get_attr_type in H1; eauto.
+          apply in_map with (f := snd) in H7.
+          eapply List.Forall_In in H5; eauto. subst; auto.
+        * eapply IHl; eauto. unfold incl in *; intuition.
+      + rewrite fst_map_fst in E2. apply inb_false_iff in E2. apply NoDup_cons; auto.
+        eapply IHl with (Gstore := Gstore); eauto.
+        unfold incl in *; intuition.
+  Qed.
 
-    Lemma In_Permuted : forall A (x : A) l', In x l' -> exists l, Permutation (x :: l) l'.
-    Proof.
-      clear. induction l'; intros.
-      - apply in_nil in H; intuition.
-      - inversion H.
-        + exists l'; subst; auto.
-        + apply IHl' in H0 as [l Hl]. exists (a :: l). eapply perm_trans; try apply perm_swap.
-          constructor; assumption.
-    Qed.
+  Lemma In_Permuted : forall A (x : A) l', In x l' -> exists l, Permutation (x :: l) l'.
+  Proof.
+    clear. induction l'; intros.
+    - apply in_nil in H; intuition.
+    - inversion H.
+      + exists l'; subst; auto.
+      + apply IHl' in H0 as [l Hl]. exists (a :: l). eapply perm_trans; try apply perm_swap.
+        constructor; assumption.
+  Qed.
 
-    Lemma double_incl_NoDup_Permuted : forall (l : list (string * expr)) (tl' : list (string * type)),
-        inclb String.eqb (List.map fst l) (List.map fst tl') = true ->
-        inclb String.eqb (List.map fst tl') (List.map fst l) = true ->
-        NoDup (List.map fst l) ->
-        length (List.map fst tl') <= length (List.map fst l) ->
-        Permutation (List.map (fun '(s, _) => (s, get_attr_type tl' s)) l) tl'.
-    Proof.
-      intros.
-      assert (NoDup (List.map fst tl')).
-      { apply inclb_correct in H, H0. eapply NoDup_incl_NoDup; eauto. }
-      generalize dependent tl'. induction l; simpl; intros.
-      - destruct tl'; simpl in *; intuition; discriminate.
-      - destruct a; simpl in *. remember (s, get_attr_type tl' s) as p.
-        rewrite Bool.andb_true_iff in H; destruct H. rewrite inb_true_iff in H.
-        assert (forall s, In s (List.map fst tl') -> In (s, get_attr_type tl' s) tl').
-        { clear; induction tl'; simpl; intros.
-          - auto.
-          - destruct a; simpl in *. destruct (String.eqb s0 s) eqn:E.
-            + rewrite String.eqb_eq in E; subst; auto.
-            + rewrite String.eqb_neq in E. right. apply IHtl'. intuition. }
-        apply H5, In_Permuted in H. destruct H as [tl Htl].
-        eapply Permutation_trans; [| apply Htl].
-        subst; apply perm_skip.
-        assert (forall (l : list (string * expr)) tl tl' s t,
-                   incl (List.map fst l) (List.map fst tl') ->
-                   Permutation ((s, t) :: tl) tl' ->
-                   ~ In s (List.map fst l) -> NoDup (List.map fst tl') ->
-                   List.map (fun '(s, _) => (s, get_attr_type tl' s)) l = List.map (fun '(s, _) => (s, get_attr_type tl s)) l).
-        { clear. induction l; simpl; intros; auto.
-          destruct a; simpl in *. f_equal.
-          - rewrite <- Permutation_NoDup_In_get_attr_type with (tl := (s,t) :: tl) (tl' := tl'); auto.
-            + simpl. destruct (String.eqb s s0) eqn:E; auto.
-              exfalso; apply H1; left; symmetry; apply String.eqb_eq; auto.
-            + intuition.
-          - eapply IHl; eauto. apply incl_cons_inv in H. intuition. }
-        erewrite H; eauto.
-        + apply IHl.
-          * inversion H1. auto.
-          * apply Permutation_sym in Htl. apply inclb_complete. apply inclb_correct in H4. auto.
-            apply Permutation_map with (f := fst) in Htl. apply Permutation_incl in Htl. unfold incl; intros.
-            apply H4 in H6 as H8. apply Htl in H8. inversion H8; auto. simpl in *; subst. inversion H1; intuition.
-          * apply inclb_complete. apply inclb_correct in H0.
-            apply Permutation_map with (f := fst) in Htl. apply Permutation_sym in Htl. apply (Permutation_NoDup Htl) in H3.
-            apply Permutation_sym in Htl. apply Permutation_incl in Htl.
-            unfold incl; intros. simpl in *. apply incl_cons_inv in Htl. apply Htl in H6 as H8. apply H0 in H8. inversion H8; auto.
-            subst. inversion H3; intuition.
-          * apply Permutation_map with (f := fst) in Htl; apply Permutation_length in Htl. simpl in Htl.
-            rewrite <- Htl in H2. apply le_S_n in H2. auto.
-          * apply Permutation_map with (f := fst) in Htl. apply Permutation_sym in Htl. apply (Permutation_NoDup Htl) in H3.
-            simpl in *. inversion H3; intuition.
-        + apply inclb_correct; auto.
-        + inversion H1; auto.
-    Qed.
-    End __.
+  Lemma Permutation_incl : forall A (l l' : list A), Permutation l l' -> incl l l'.
+  Proof.
+    intros. unfold incl; intros.
+    eapply Permutation_in; eauto.
+  Qed.
 
-    Lemma proj_record_type_sound : forall l s t, proj_record_type l s = Success t -> In (s, t) l.
-    Proof.
-      induction l; simpl in *; try discriminate. intros.
-      destruct a. destruct_match; auto.
-      rewrite String.eqb_eq in E. invert_result. auto.
-    Qed.
+  Lemma double_incl_NoDup_Permuted : forall (l : list (string * expr)) (tl' : list (string * type)),
+      inclb String.eqb (List.map fst l) (List.map fst tl') = true ->
+      inclb String.eqb (List.map fst tl') (List.map fst l) = true ->
+      NoDup (List.map fst l) ->
+      length (List.map fst tl') <= length (List.map fst l) ->
+      Permutation (List.map (fun '(s, _) => (s, get_attr_type tl' s)) l) tl'.
+  Proof.
+    intros.
+    assert (NoDup (List.map fst tl')).
+    { apply inclb_correct in H, H0. eapply NoDup_incl_NoDup; eauto. }
+    generalize dependent tl'. induction l; simpl; intros.
+    - destruct tl'; simpl in *; intuition; discriminate.
+    - destruct a; simpl in *. remember (s, get_attr_type tl' s) as p.
+      rewrite Bool.andb_true_iff in H; destruct H. rewrite inb_true_iff in H.
+      assert (forall s, In s (List.map fst tl') -> In (s, get_attr_type tl' s) tl').
+      { clear; induction tl'; simpl; intros.
+        - auto.
+        - destruct a; simpl in *. destruct (String.eqb s0 s) eqn:E.
+          + rewrite String.eqb_eq in E; subst.
+            unfold get_attr_type, access_record. rewrite eqb_refl; auto.
+          + rewrite String.eqb_neq in E. right. apply not_eq_sym in E as E'. rewrite <- eqb_neq in E'.
+            unfold get_attr_type, access_record. rewrite E'. apply IHtl'. intuition. }
+      apply H5, In_Permuted in H. destruct H as [tl Htl].
+      eapply Permutation_trans; [| apply Htl].
+      subst; apply perm_skip.
+      assert (forall (l : list (string * expr)) tl tl' s t,
+                 incl (List.map fst l) (List.map fst tl') ->
+                 Permutation ((s, t) :: tl) tl' ->
+                 ~ In s (List.map fst l) -> NoDup (List.map fst tl') ->
+                 List.map (fun '(s, _) => (s, get_attr_type tl' s)) l = List.map (fun '(s, _) => (s, get_attr_type tl s)) l).
+      { generalize dependent width; generalize dependent tenv; clear; intros. induction l; simpl; intros; auto.
+        destruct a; simpl in *. f_equal.
+        - rewrite <- Permutation_NoDup_In_get_attr_type with (tl := (s,t) :: tl) (tl' := tl'); auto.
+          + simpl. destruct (String.eqb s s0) eqn:E.
+            * exfalso; apply H1; left; symmetry; apply String.eqb_eq; auto.
+            * unfold get_attr_type. simpl. rewrite eqb_sym, E. auto.
+          + intuition.
+        - eapply IHl; eauto. apply incl_cons_inv in H. intuition. }
+      erewrite H; eauto.
+      + apply IHl.
+        * inversion H1. auto.
+        * apply Permutation_sym in Htl. apply inclb_complete. apply inclb_correct in H4. auto.
+          apply Permutation_map with (f := fst) in Htl. apply Permutation_incl in Htl. unfold incl; intros.
+          apply H4 in H6 as H8. apply Htl in H8. inversion H8; auto. simpl in *; subst. inversion H1; intuition.
+        * apply inclb_complete. apply inclb_correct in H0.
+          apply Permutation_map with (f := fst) in Htl. apply Permutation_sym in Htl. apply (Permutation_NoDup Htl) in H3.
+          apply Permutation_sym in Htl. apply Permutation_incl in Htl.
+          unfold incl; intros. simpl in *. apply incl_cons_inv in Htl. apply Htl in H6 as H8. apply H0 in H8. inversion H8; auto.
+          subst. inversion H3; intuition.
+        * apply Permutation_map with (f := fst) in Htl; apply Permutation_length in Htl. simpl in Htl.
+          rewrite <- Htl in H2. apply le_S_n in H2. auto.
+        * apply Permutation_map with (f := fst) in Htl. apply Permutation_sym in Htl. apply (Permutation_NoDup Htl) in H3.
+          simpl in *. inversion H3; intuition.
+      + apply inclb_correct; auto.
+      + inversion H1; auto.
+  Qed.
 
+  Lemma access_record_sound : forall A l s (a : A), access_record l s = Success a -> In (s, a) l.
+  Proof.
+    induction l; simpl in *; try discriminate. intros.
+    destruct a. destruct_match; auto.
+    rewrite String.eqb_eq in E. invert_result. auto.
+  Qed.
+
+(*
     Lemma dict_from'_sound : forall l,
         Forall (fun p =>
                   (forall (Gstore Genv : tenv) (t : type) (e' : expr),
@@ -266,7 +321,79 @@ Section WithWord.
           * apply H2 in E4. apply E4.
         + eapply IHl; eauto.
     Qed.
+ *)
 
+  Lemma first_success_exists_l : forall Gstore Genv t l,
+      first_success (List.map (fun '(k, _) => synthesize_expr Gstore Genv k) l) = Success t ->
+      exists (p : expr * expr) e, In p l /\ synthesize_expr Gstore Genv (fst p) = Success (t, e).
+  Proof.
+    induction l; simpl; intros; try discriminate.
+    destruct a as [k v]. destruct_match.
+    - destruct a; invert_result; subst. eauto.
+    - apply IHl in H as [p [e H]]. exists p; exists e. intuition.
+  Qed.
+
+  Lemma first_success_exists_r : forall Gstore Genv t l,
+      first_success (List.map (fun '(_, v) => synthesize_expr Gstore Genv v) l) = Success t ->
+      exists (p : expr * expr) e, In p l /\ synthesize_expr Gstore Genv (snd p) = Success (t, e).
+  Proof.
+    induction l; simpl; intros; try discriminate.
+    destruct a as [k v]. destruct_match.
+    - destruct a; invert_result; subst. eauto.
+    - apply IHl in H as [p [e H]]. exists p; exists e. intuition.
+  Qed.
+
+  Lemma dict_from'_sound : forall l,
+      Forall (fun p =>
+                (forall (Gstore Genv : tenv) (t : type) (e' : expr),
+                    tenv_wf Gstore ->
+                    tenv_wf Genv ->
+                    (synthesize_expr Gstore Genv (fst p) = Success (t, e') -> type_of Gstore Genv (fst p) t) /\
+                      (analyze_expr Gstore Genv t (fst p) = Success e' -> type_wf t -> type_of Gstore Genv (fst p) t)) /\
+                  (forall (Gstore Genv : tenv) (t : type) (e' : expr),
+                      tenv_wf Gstore ->
+                      tenv_wf Genv ->
+                      (synthesize_expr Gstore Genv (snd p) = Success (t, e') -> type_of Gstore Genv (snd p) t) /\
+                        (analyze_expr Gstore Genv t (snd p) = Success e' -> type_wf t  -> type_of Gstore Genv (snd p) t))) l ->
+      forall Gstore Genv kt vt l',
+        tenv_wf Gstore -> tenv_wf Genv ->
+        type_wf kt -> type_wf vt ->
+        dict_from' (List.map (fun '(k, v) => k' <- analyze_expr Gstore Genv kt k;; v' <- analyze_expr Gstore Genv vt v;; Success (k', v')) l) = Success l' -> Forall (fun p => type_of Gstore Genv (fst p) kt /\ type_of Gstore Genv (snd p) vt) l.
+  Proof.
+   Proof.
+      induction l; simpl; intros.
+      - apply Forall_nil.
+      - repeat destruct_match. invert_result. inversion H; subst; simpl in *.
+        constructor.
+        + split; simpl.
+          * apply H6 in E3; auto.
+          * apply H6 in E4; auto.
+        + eapply IHl; eauto.
+   Qed.
+
+  Lemma analyze_dict_body_sound : forall l,
+      Forall (fun p =>
+                (forall (Gstore Genv : tenv) (t : type) (e' : expr),
+                    tenv_wf Gstore ->
+                    tenv_wf Genv ->
+                    (synthesize_expr Gstore Genv (fst p) = Success (t, e') -> type_of Gstore Genv (fst p) t) /\
+                      (analyze_expr Gstore Genv t (fst p) = Success e' -> type_wf t -> type_of Gstore Genv (fst p) t)) /\
+                  (forall (Gstore Genv : tenv) (t : type) (e' : expr),
+                      tenv_wf Gstore ->
+                      tenv_wf Genv ->
+                      (synthesize_expr Gstore Genv (snd p) = Success (t, e') -> type_of Gstore Genv (snd p) t) /\
+                        (analyze_expr Gstore Genv t (snd p) = Success e' -> type_wf t -> type_of Gstore Genv (snd p) t))) l ->
+      forall Gstore Genv kt vt e',
+        tenv_wf Gstore -> tenv_wf Genv ->
+        type_wf kt -> type_wf vt ->
+        analyze_dict_body analyze_expr Gstore Genv kt vt l = Success e' -> Forall (fun p => type_of Gstore Genv (fst p) kt /\ type_of Gstore Genv (snd p) vt) l.
+  Proof.
+      unfold analyze_dict_body, dict_from. intros.
+      destruct_match. invert_result.
+      eapply dict_from'_sound; eauto.
+    Qed.
+
+  (*
     Lemma analyze_dict_body_sound : forall l,
         Forall (fun p =>
                   (forall (Gstore Genv : tenv) (t : type) (e' : expr),
@@ -281,21 +408,56 @@ Section WithWord.
       unfold analyze_dict_body, dict_from. intros.
       destruct_match. invert_result. eapply dict_from'_sound; eauto.
     Qed.
+ *)
 
-    Local Ltac unfold_typechecker := lazymatch goal with
-                               | H: context [synthesize_expr _ _ ?e] |- _ => unfold synthesize_expr in H
-                               | H: context [analyze_expr _ _ _ ?e] |- _ => unfold analyze_expr in H
-                               end.
+  Local Ltac unfold_typechecker :=
+    lazymatch goal with
+    | H: context [synthesize_expr _ _ ?e] |- _ => unfold synthesize_expr in H
+    | H: context [analyze_expr _ _ _ ?e] |- _ => unfold analyze_expr in H
+    end.
 
-    Local Ltac unfold_fold_typechecker := repeat unfold_typechecker; fold synthesize_expr in *; fold analyze_expr in *.
+  Local Ltac unfold_fold_typechecker := repeat unfold_typechecker; fold synthesize_expr in *; fold analyze_expr in *.
+
+  Ltac apply_type_of__type_wf :=
+    lazymatch goal with
+    | H: type_of _ _ _ ?t |- type_wf ?t =>
+        let H' := fresh "H'" in
+        apply type_of__type_wf in H as H'
+    | H: type_of _ _ _ (TList ?t) |- type_wf ?t =>
+        let H' := fresh "H'" in
+        apply type_of__type_wf in H as H'
+    | H:  type_of _ _ _ (TOption ?t) |- type_wf ?t =>
+        let H' := fresh "H'" in
+        apply type_of__type_wf in H as H'
+    | H:  type_of _ _ _ (TDict ?t _) |- type_wf ?t =>
+        let H' := fresh "H'" in
+        apply type_of__type_wf in H as H'
+    | H:  type_of _ _ _ (TDict _ ?t) |- type_wf ?t =>
+        let H' := fresh "H'" in
+        apply type_of__type_wf in H as H'
+    | H:  type_of _ _ _ (TRecord ?tl) |- context[?tl] =>
+        let H' := fresh "H'" in
+        apply type_of__type_wf in H as H'
+    end.
+
+  Local Ltac apply_typechecker_IH :=
+    lazymatch goal with
+    | IH: (forall _ _ _ _, _ -> _ -> (synthesize_expr _ _ ?e = _ -> _) /\ _),
+        H: synthesize_expr _ _ ?e = Success _ |- context[?e] => eapply IH in H; eauto
+    | IH: (forall _ _ _ _, _ -> _ -> _ /\ (analyze_expr _ _ _ ?e = _ -> _)),
+        H: analyze_expr _ _ _ ?e = Success _ |- context[?e] => eapply IH in H; eauto
+    | IH: (forall _ _ _ _, _ -> _ -> (synthesize_expr _ _ ?e = _ -> _) /\ _),
+        H: synthesize_expr _ _ ?e = Success (?t, _) |- context[?t] => eapply IH in H; eauto
+    | IH: (forall _ _ _ _, _ -> _ -> _ /\ (analyze_expr _ _ _ ?e = _ -> _)),
+        H: analyze_expr _ _ ?t ?e = Success _ |- context[?t] => eapply IH in H; eauto
+    end.
 
     Lemma typechecker_sound : forall e Gstore Genv t e',
+        tenv_wf Gstore -> tenv_wf Genv ->
         (synthesize_expr Gstore Genv e = Success (t, e') -> type_of Gstore Genv e t) /\
-          (analyze_expr Gstore Genv t e = Success e' -> type_of Gstore Genv e t).
+          (analyze_expr Gstore Genv t e = Success e' -> type_wf t -> type_of Gstore Genv e t).
     Proof.
-      apply (expr_IH (fun e => forall (Gstore Genv : tenv) (t : type) (e' : expr),
-  (synthesize_expr Gstore Genv e = Success (t, e') -> type_of Gstore Genv e t) /\
-  (analyze_expr Gstore Genv t e = Success e' -> type_of Gstore Genv e t))); intros.
+      induction e using expr_IH; intros.
       - (* EVar *)
         split; intros; unfold_fold_typechecker; repeat destruct_match; invert_result; constructor; easy.
       - (* ELoc *)
@@ -305,73 +467,129 @@ Section WithWord.
           invert_result; apply atom_typechecker_sound in E; auto.
       - (* EUnop *)
         split; intros; destruct o; simpl in *;
-          try (unfold_fold_typechecker; repeat destruct_match; try invert_result; apply_typechecker_IH;
-               try invert_pair; repeat econstructor; eauto).
+          unfold_fold_typechecker; repeat destruct_match; try invert_result;
+          apply_typechecker_IH; try invert_pair; repeat (econstructor; eauto);
+          try apply_type_of__type_wf; auto; invert_type_wf; auto.
       - (* EBinop *)
         split; intros; destruct o; simpl in *;
-          try (unfold_fold_typechecker; repeat destruct_match; try invert_result; repeat apply_typechecker_IH;
-               try invert_pair; repeat econstructor; eauto).
+        unfold_fold_typechecker; repeat destruct_match; try invert_result;
+        repeat (apply_typechecker_IH; try invert_pair; try econstructor; eauto; try constructor;
+                try apply_type_of__type_wf; auto; try invert_type_wf; auto).
       - (* EIf *)
         split; intros; unfold_fold_typechecker; repeat destruct_match;
-          repeat apply_typechecker_IH; invert_result; econstructor; eauto.
+          repeat (apply_typechecker_IH; try invert_result; try econstructor; eauto;
+                try apply_type_of__type_wf; auto; try invert_type_wf; auto).
       - (* ELet *)
         split; intros; unfold_fold_typechecker; repeat destruct_match;
-          repeat apply_typechecker_IH; invert_result; econstructor; eauto.
+          repeat (try apply_typechecker_IH; try invert_result; try econstructor; eauto;
+                  try apply_type_of__type_wf; auto; try invert_type_wf; auto;
+                  try apply tenv_wf_step; auto).
       - (* EFlatmap *)
-        split; intros; unfold_fold_typechecker; repeat destruct_match; repeat apply_typechecker_IH; invert_result; econstructor; eauto.
+        split; intros; unfold_fold_typechecker; repeat destruct_match;
+          repeat (try apply_typechecker_IH; try invert_result; try econstructor; eauto;
+                  try apply_type_of__type_wf; auto; try invert_type_wf; auto;
+                  try apply tenv_wf_step; auto).
       - (* EFold *)
-        split; intros; unfold_fold_typechecker; repeat destruct_match; repeat apply_typechecker_IH; invert_result; econstructor; eauto.
+        split; intros; unfold_fold_typechecker; repeat destruct_match;
+          repeat (try apply_typechecker_IH; try invert_result; try econstructor; eauto;
+                  try apply_type_of__type_wf; auto; try invert_type_wf; auto;
+                  try apply tenv_wf_step; auto).
       - (* ERecord *)
         split; intros; unfold_fold_typechecker; repeat destruct_match.
         + unfold record_type_from in *. repeat destruct_match. invert_result.
-          pose proof record_type_from'_sound. eapply H0 in H; eauto.
-          apply TyERecord with (tl := l0); intuition;
-          [ apply Permuted_record_sort | apply StronglySorted_record_sort ].
-        + assert (type_eqb (TRecord l0) (TRecord (record_sort l0))); auto.
-          apply type_eqb_eq in H1. injection H1; intro. unfold record_from in *. destruct_match. invert_result.
-          pose proof record_from'_sound. eapply H0 in H; eauto.
+          eapply record_type_from'_sound with (Gstore := Gstore) (Genv := Genv) in H; eauto.
+          apply TyERecord with (tl := l0); intuition.
+          * apply Permuted_record_sort.
+          * rewrite <- H2; auto.
+          * apply StronglySorted_record_sort.
+        + unfold record_from in *. destruct_match. invert_result.
+          rewrite Bool.andb_true_iff in E1. intuition.
+          eapply record_from'_sound with (Gstore := Gstore) in H; eauto; [| apply inclb_correct; auto].
           apply TyERecord with (tl := List.map (fun '(s, e) => (s, get_attr_type l0 s)) l); intuition.
-          * rewrite Bool.andb_true_iff in E2. apply double_incl_NoDup_Permuted; intuition.
+          * apply double_incl_NoDup_Permuted; intuition.
             apply leb_complete. repeat rewrite map_length. auto.
-          * rewrite H2. apply StronglySorted_record_sort.
+          * rewrite fst_map_fst; auto.
+          * inversion H3; auto.
       - (* EAccess *)
-        split; intros; unfold_fold_typechecker; repeat destruct_match; repeat apply_typechecker_IH; invert_result; econstructor; eauto;
-          auto using proj_record_type_sound.
+        split; intros; unfold_fold_typechecker; repeat destruct_match;
+          repeat (apply_typechecker_IH; try invert_result; try econstructor; eauto;
+                  try apply_type_of__type_wf; auto; try invert_type_wf; auto).
       - (* EDict *)
-        split; intros; unfold_fold_typechecker; repeat destruct_match; try invert_result; constructor;
-        eapply analyze_dict_body_sound; eauto.
+        split; intros; unfold_fold_typechecker; repeat destruct_match;
+          repeat (apply_typechecker_IH; try invert_result; try econstructor; eauto;
+                  try apply_type_of__type_wf; auto; try invert_type_wf; auto).
+        + invert_result. constructor.
+          * apply first_success_exists_l in E as [p0 [e0 [HL HR]]]. rewrite Forall_forall in H.
+            apply H in HR; auto; apply_type_of__type_wf; auto.
+          * apply first_success_exists_r in E0 as [p0 [e0 [HL HR]]]. rewrite Forall_forall in H.
+            apply H in HR; auto; apply_type_of__type_wf; auto.
+          * eapply analyze_dict_body_sound; eauto.
+            -- apply first_success_exists_l in E as [p0 [e0 [HL HR]]]. rewrite Forall_forall in H.
+               apply H in HR; auto; apply_type_of__type_wf; auto.
+            -- apply first_success_exists_r in E0 as [p0 [e0 [HL HR]]]. rewrite Forall_forall in H.
+               apply H in HR; auto; apply_type_of__type_wf; auto.
+        + constructor; try invert_type_wf; auto.
+          eapply analyze_dict_body_sound; eauto; invert_type_wf; auto.
       - (* EInsert *)
-        split; intros; unfold_fold_typechecker; repeat destruct_match; repeat apply_typechecker_IH; invert_result; constructor; auto.
+        split; intros; unfold_fold_typechecker; repeat destruct_match;
+          repeat (apply_typechecker_IH; try invert_result; try apply_type_of__type_wf; auto;
+                  try invert_type_wf; auto; try econstructor; eauto).
       - (* EDelete *)
-        split; intros; unfold_fold_typechecker; repeat destruct_match; repeat apply_typechecker_IH; invert_result; constructor; auto.
+        split; intros; unfold_fold_typechecker; repeat destruct_match;
+          repeat (apply_typechecker_IH; try invert_result; try apply_type_of__type_wf; auto;
+                  try invert_type_wf; auto; try econstructor; eauto).
       - (* ELookup *)
-        split; intros; unfold_fold_typechecker; repeat destruct_match; repeat apply_typechecker_IH; invert_result; econstructor; eauto.
+        split; intros; unfold_fold_typechecker; repeat destruct_match;
+          repeat (apply_typechecker_IH; try invert_result; try apply_type_of__type_wf; auto;
+                  try invert_type_wf; auto; try econstructor; eauto).
+      - (* EOptmatch *)
+        split; intros; unfold_fold_typechecker; repeat destruct_match;
+          repeat (try apply_typechecker_IH; try invert_result; try apply_type_of__type_wf; auto;
+                  try apply tenv_wf_step; try invert_type_wf; auto;
+                  try invert_type_wf; auto; try econstructor; eauto).
       - (* EFilter *)
-        split; intros; unfold_fold_typechecker; repeat destruct_match; repeat apply_typechecker_IH; invert_result; econstructor; eauto.
+        split; intros; unfold_fold_typechecker; repeat destruct_match;
+          repeat (try apply_typechecker_IH; try invert_result; try apply_type_of__type_wf; auto;
+                  try apply tenv_wf_step; try invert_type_wf; auto;
+                  try invert_type_wf; auto; try econstructor; eauto).
       - (* EJoin *)
-        split; intros; unfold_fold_typechecker; repeat destruct_match; repeat apply_typechecker_IH; invert_result; econstructor; eauto.
+        split; intros; unfold_fold_typechecker; repeat destruct_match;
+          repeat (try apply_typechecker_IH; try invert_result; try apply_type_of__type_wf; auto;
+                  try repeat apply tenv_wf_step; try invert_type_wf; auto;
+                  try invert_type_wf; auto; try econstructor; eauto).
+        all: apply IHe2 in E2; auto; apply_type_of__type_wf; auto; invert_type_wf; auto.
       - (* EProj *)
-        split; intros; unfold_fold_typechecker; repeat destruct_match; repeat apply_typechecker_IH; invert_result; econstructor; eauto.
+        split; intros; unfold_fold_typechecker; repeat destruct_match;
+          repeat (try apply_typechecker_IH; try invert_result; try apply_type_of__type_wf; auto;
+                  try repeat apply tenv_wf_step; try invert_type_wf; auto;
+                  try invert_type_wf; auto; try econstructor; eauto).
     Qed.
 
     Local Ltac apply_type_sound_IH :=
       lazymatch goal with
-      | H : (forall store env, well_formed_locals ?Gstore store ->
-                               well_formed_locals ?Genv env -> _),
-          H1: well_formed_locals ?Gstore _,
-            H2: well_formed_locals ?Genv _ |- _ =>
+      | H : (tenv_wf ?Genv ->
+             forall store env, locals_wf ?Gstore store ->
+                               locals_wf ?Genv env -> _),
+          H0: tenv_wf ?Genv,
+          H1: locals_wf ?Gstore _,
+            H2: locals_wf ?Genv _ |- _ =>
           let H' := fresh "H'" in
-          pose proof (H _ _ H1 H2) as H'; clear H; inversion H'; subst
-      | H : (forall _ _, _ -> _ -> type_of_value (interp_expr _ _ ?e) ?t) |- type_of_value (interp_expr _ _ ?e) ?t =>
-          apply H; try apply well_formed_locals_step
+          pose proof (H H0 _ _ H1 H2) as H'; clear H; inversion H'; subst
+      | H : (tenv_wf ?Genv0 ->
+             forall _ _, _ -> _ -> type_of_value (interp_expr _ _ ?e) ?t) |- type_of_value (interp_expr _ _ ?e) ?t =>
+          apply H; try apply tenv_wf_step; try apply locals_wf_step
       end.
 
-    Local Ltac apply_well_formed_locals :=
+    Local Ltac type_injection :=
+      lazymatch goal with
+      | H : TList _ = TList _ |- _ => injection H as H; subst
+      end.
+
+    Local Ltac apply_locals_wf :=
       match goal with
-      | H : well_formed_locals ?G ?E, H' : map.get ?G ?x = _ |- _ =>
+      | H : locals_wf ?G ?E, H' : map.get ?G ?x = _ |- _ =>
           apply H in H'; unfold get_local; destruct (map.get E x); intuition
       end.
-
     Local Ltac invert_Forall :=
       match goal with
       | H : Forall _ (_ :: _) |- _ => inversion H; subst
@@ -381,6 +599,7 @@ Section WithWord.
       match goal with
       | H: exists x, _ |- _ => destruct H as [x H]
       end.
+
 
     Lemma Forall2_In_Permuted : forall A B (R : A -> B -> Prop) l1 l2 a, Forall2 R l1 l2 -> In a l1 -> exists l1_0 b l2_0, Permutation l1 (a :: l1_0) /\ Permutation l2 (b :: l2_0) /\ R a b /\ Forall2 R l1_0 l2_0.
     Proof.
@@ -392,13 +611,6 @@ Section WithWord.
           exists (x :: l1_0), b, (y :: l2_0); intuition.
           * apply Permutation_trans with (l' := x :: a :: l1_0); auto using perm_swap.
           * apply Permutation_trans with (l' := y :: b :: l2_0); auto using perm_swap.
-    Qed.
-
-    Lemma In_fst : forall A B x (l : list (A * B)), In x (List.map fst l) -> exists p, In p l /\ fst p = x.
-    Proof.
-      induction l; simpl; intros; intuition.
-      - exists a. intuition.
-      - destruct H as [p H]; exists p; intuition.
     Qed.
 
     Lemma Forall2_Permuted_StronglySorted : forall A B R (l1 : list (string * A)) (l2 : list (string * B)) l1' l2',
@@ -468,11 +680,12 @@ Section WithWord.
       - inversion H; intuition.
     Qed.
 
-    Lemma TyVDict_def : forall l tk tv, Forall (fun p => type_of_value (fst p) tk /\ type_of_value (snd p) tv) l <-> type_of_value (VDict l) (TDict tk tv).
+    Lemma TyVDict_def : forall l kt vt, type_wf kt -> type_wf vt ->
+                                        Forall (fun p => type_of_value (fst p) kt /\ type_of_value (snd p) vt) l <-> type_of_value (VDict l) (TDict kt vt).
     Proof.
       split; intros.
       - constructor; auto.
-      - inversion H; intuition.
+      - inversion H1; intuition.
     Qed.
 
     Lemma record_proj_sound : forall l, NoDup (List.map fst l) ->
@@ -491,42 +704,50 @@ Section WithWord.
     Qed.
 
     Lemma dict_insert_sound : forall l kt vt k v,
+        type_wf kt -> type_wf vt ->
         type_of_value (VDict l) (TDict kt vt) ->
         type_of_value k kt ->
         type_of_value v vt ->
         type_of_value (VDict (dict_insert k v l)) (TDict kt vt).
     Proof.
-      intros. induction l; constructor; simpl.
-      - constructor; intuition.
-      - destruct a as [k' v']. destruct (value_ltb k k'); [| destruct(value_eqb k k')]; inversion H.
-        + auto.
-        + inversion H4; auto.
-        + inversion H4; subst; constructor; intuition.
-          rewrite TyVDict_def. apply IHl. constructor. inversion H. intuition.
+      intros. induction l; constructor; simpl; auto.
+      destruct a as [k' v']. destruct (value_ltb k k'); [| destruct(value_eqb k k')];
+        match goal with
+        | H: type_of_value (VDict (_ :: _)) _ |- _ => inversion H; subst
+        end; auto.
+        + invert_Forall; auto.
+        + invert_Forall; subst; constructor; intuition.
+          rewrite TyVDict_def; auto. apply IHl. constructor; auto.
     Qed.
 
     Lemma dict_delete_sound : forall l kt vt k,
+        type_wf kt -> type_wf vt ->
         type_of_value (VDict l) (TDict kt vt) ->
         type_of_value k kt ->
         type_of_value (VDict (dict_delete k l)) (TDict kt vt).
     Proof.
-      intros; induction l; constructor; simpl.
-      - constructor.
-      - destruct a as [k' v']. destruct (value_eqb k k'); inversion H; inversion H3.
-        + auto.
-        + constructor; auto. try rewrite TyVDict_def in *. apply IHl; auto.
+      intros; induction l; constructor; simpl; auto.
+      destruct a as [k' v']. destruct (value_eqb k k');
+       match goal with
+        | H: type_of_value (VDict (_ :: _)) _ |- _ => inversion H; subst
+        end; invert_Forall; auto.
+      constructor; auto. try rewrite TyVDict_def in *; auto.
     Qed.
 
     Lemma dict_lookup_sound : forall l kt vt k,
+        type_wf kt -> type_wf vt ->
         type_of_value (VDict l) (TDict kt vt) ->
         type_of_value k kt ->
         type_of_value (VOption (dict_lookup k l)) (TOption vt).
     Proof.
       intros; induction l.
       - constructor.
-      - simpl. destruct a as [k' v']. destruct (value_eqb k k').
-        + constructor. inversion H; inversion H3. intuition.
-        + apply IHl. constructor. inversion H; inversion H3. auto.
+      - simpl. destruct a as [k' v']. destruct (value_eqb k k');
+          match goal with
+          | H: type_of_value (VDict (_ :: _)) _ |- _ => inversion H; subst
+          end; invert_Forall; auto.
+        + constructor. intuition.
+        + apply IHl. constructor; auto.
     Qed.
 
     Lemma Forall_Forall_filter : forall A P (l : list A), Forall P l -> forall f, Forall P (filter f l).
@@ -557,25 +778,20 @@ Section WithWord.
       - rewrite TyVList_def. eapply IHl; eauto. constructor. auto.
     Qed.
 
-    Lemma type_sound : forall Gstore Genv e t,
-        type_of Gstore Genv e t ->
-        forall store env,
-        well_formed_locals Gstore store ->
-        well_formed_locals Genv env ->
+  Lemma type_sound : forall Gstore Genv e t,
+      type_of Gstore Genv e t ->
+      tenv_wf Gstore -> tenv_wf Genv ->
+      forall store env,
+        locals_wf Gstore store -> locals_wf Genv env ->
         type_of_value (interp_expr store env e) t.
     Proof.
-      intros Gstore Genv e t H. apply (type_of_IH Gstore) with
-        (P := fun Genv e t => forall store env,
-        well_formed_locals Gstore store ->
-        well_formed_locals Genv env ->
-        type_of_value (interp_expr store env e) t); simpl; intros; auto.
-      - apply_well_formed_locals.
-      - apply_well_formed_locals.
-      - match goal with H : type_of_atom _ _ |- _ => inversion H end; subst; constructor; apply Forall_nil.
-      - inversion H0; subst; apply_type_sound_IH;
-          simpl; repeat constructor; auto.
-      - inversion H0; subst; repeat apply_type_sound_IH;
-          simpl; repeat constructor; auto.
+      intros Gstore Genv e t H H_Gstore H_Genv. induction H using @type_of_IH; simpl; intros store env H_store H_env; auto.
+      1, 2: (* TyEVar | TyELoc *)
+        apply_locals_wf.
+      - (* TyEAtom *)
+        match goal with H : type_of_atom _ _ |- _ => inversion H end; subst; constructor; apply Forall_nil.
+      - inversion H; apply_type_sound_IH; try discriminate; repeat constructor; auto.
+      - inversion H; repeat apply_type_sound_IH; try discriminate; try type_injection; repeat constructor; auto.
         + apply Forall_app; auto.
         + assert (forall A f (l : list A), Forall f l -> forall n, Forall f (concat (repeat l n))).
           { clear. induction n; simpl; intros.
@@ -593,77 +809,89 @@ Section WithWord.
             - repeat constructor; auto. }
           auto.
       - repeat apply_type_sound_IH;
-        match goal with
-        | |- type_of_value (if ?b then _ else _) _ => destruct b; constructor; auto
-        end.
-      - repeat apply_type_sound_IH; auto; constructor; auto.
-      - repeat apply_type_sound_IH.
+          match goal with
+          | |- type_of_value (if ?b then _ else _) _ => destruct b; constructor; auto
+          end.
+      - repeat apply_type_sound_IH; try constructor;
+          try apply_type_of__type_wf; try invert_type_wf; auto.
+      - repeat apply_type_sound_IH;
         clear H1. constructor. induction l; simpl.
         + apply Forall_nil.
         + apply Forall_app; split.
           * invert_Forall.
             assert (type_of_value (interp_expr store (map.put env x a) e2) (TList t2)).
-            { apply_type_sound_IH; auto. }
+            { apply_type_sound_IH; auto. apply type_of__type_wf in H; try invert_type_wf; auto. }
             inversion H1; auto.
-          * apply IHl. inversion H7. assumption.
+          * apply IHl. inversion H3. assumption.
       - repeat apply_type_sound_IH;
           try (match goal with
                | H: VList ?l = _ |- _ => clear H
                end; induction l; simpl; try constructor; auto; apply_type_sound_IH; auto;
                match goal with
                | H: Forall _ (_ :: _) |- _ => inversion H; subst
-               end;
-             repeat apply well_formed_locals_step; auto);
-          try (clear H1; induction l0; simpl; try constructor; auto;
-           apply_type_sound_IH; auto;
-           match goal with
-           | H: Forall _ (_ :: _) |- _ => inversion H; subst
-           end;
-           repeat apply well_formed_locals_step; auto).
-      - constructor.
-        + apply Permutation_NoDup with (l := List.map fst (List.map (fun '(s, e0) => (s, interp_expr store env e0)) l)).
-          * apply Permutation_map. apply Permuted_record_sort.
-          * rewrite fst_map_fst. auto.
-        + apply StronglySorted_record_sort.
+               end);
+               repeat apply locals_wf_step; auto; repeat apply tenv_wf_step; auto;
+          try apply_type_of__type_wf; try invert_type_wf; auto.
+        all: match goal with
+             | H: VList ?l = _ |- type_of_value (fold_right _ _ ?l) _ => clear H; induction l end;
+          simpl; try constructor; auto; apply_type_sound_IH; auto;
+          match goal with
+          | H: Forall _ (_ :: _) |- _ => inversion H; subst
+          end;
+          repeat apply locals_wf_step; auto; repeat apply tenv_wf_step; auto;
+          try apply_type_of__type_wf; try invert_type_wf; auto.
+      - constructor; auto.
+        + apply Permutation_NoDup with (l := List.map fst tl); auto. apply Permutation_map; auto.
         + remember (fun p tp => fst p = fst tp /\ type_of_value (snd p) (snd tp)) as R.
           assert (Forall2 R (List.map (fun '(s, e0) => (s, interp_expr store env e0)) l) tl).
-          { generalize dependent H0; generalize dependent H2; generalize dependent H6; generalize dependent H7; generalize dependent HeqR.
-            clear. intros H0 H1 H2 H3 H4. generalize dependent tl.
+          { revert H_Genv H_store H_env H H1 HeqR. clear; intros; generalize dependent tl.
             induction l; simpl; intros; destruct tl; try discriminate.
             - intuition.
             - destruct a, p; simpl in *; subst. constructor.
-              + simpl. split; try congruence. inversion H3; subst. apply H6; auto.
-              + apply IHl; inversion H3; inversion H4; intuition.
-          }
+              + simpl. split; try congruence. inversion H1; auto.
+              + apply IHl; inversion H; inversion H1; intuition. }
           eapply Forall2_Permuted_StronglySorted; eauto.
-          * rewrite fst_map_fst; auto.
+          * rewrite fst_map_fst; rewrite H; auto.
           * subst; intuition.
           * apply Permuted_record_sort.
           * apply StronglySorted_record_sort.
       - repeat apply_type_sound_IH. eapply record_proj_sound; eauto.
-      - constructor. rewrite Forall_forall in *.
-
+        + rewrite <- H1 in *. assert (E: List.map fst l = List.map fst tl).
+          { revert H5; clear; intros H5. induction H5; simpl; auto.
+            intuition; congruence. }
+          rewrite E; auto.
+        + apply access_record_sound; auto.
+      - constructor; auto. rewrite Forall_forall in *.
         assert (forall p, In p (List.map (fun '(k, v) => (interp_expr store env k, interp_expr store env v)) l) -> type_of_value (fst p) kt /\ type_of_value (snd p) vt).
-         { induction l; intros; simpl in *; try now (exfalso; auto).
-           inversion H4.
-           - pose proof (H1 a). intuition; destruct a; subst; simpl in *;
-               try apply H4; try apply H9; auto.
+        { induction l; intros; simpl in *; try now (exfalso; auto).
+          destruct H3.
+          - pose proof (H1 a); intuition; destruct a; subst; simpl in *.
+            + change e with (fst (e, e0)). apply H2; auto.
+            + change e0 with (snd (e, e0)). apply H2; auto.
            - apply IHl; auto. }
-        intros. apply H4. pose proof (Permuted_dict_sort (width:=width)).
+        intros. apply H3. pose proof (Permuted_dict_sort (width:=width)).
         eapply Permutation_in; [ apply Permutation_sym |]; eauto.
-      - repeat apply_type_sound_IH; apply dict_insert_sound; constructor; auto.
-      - repeat apply_type_sound_IH; apply dict_delete_sound; constructor; auto.
-      - repeat apply_type_sound_IH; eapply dict_lookup_sound; econstructor; eauto.
+      - repeat apply_type_sound_IH; apply dict_insert_sound; constructor; try invert_type_wf; auto.
+      - repeat apply_type_sound_IH; apply dict_delete_sound; try constructor;
+          try apply_type_of__type_wf; try invert_type_wf; auto.
+      - repeat apply_type_sound_IH;
+          lazymatch goal with
+          | H: Forall (fun p => type_of_value (fst p) ?t /\ _) _ |- _ => apply dict_lookup_sound with (kt := t)
+          end; try constructor; try invert_type_wf; auto.
+      - repeat apply_type_sound_IH; auto; try constructor;
+          try apply_type_of__type_wf; try invert_type_wf; auto.
       - repeat apply_type_sound_IH. constructor. apply Forall_Forall_filter. auto.
       - repeat apply_type_sound_IH.
-        rewrite <- H1 in H'0. eapply flat_map_type_sound; eauto. intros.
+        rewrite <- H4 in H'0. eapply flat_map_type_sound; eauto. intros.
         apply map_type_sound with (t := t2).
         + constructor; apply Forall_Forall_filter; auto.
-        + intuition. repeat apply_type_sound_IH; repeat apply well_formed_locals_step; auto.
+        + intuition. repeat apply_type_sound_IH; repeat apply locals_wf_step; auto;
+            try apply tenv_wf_step; try apply_type_of__type_wf; try invert_type_wf; auto.
       - repeat apply_type_sound_IH.
         apply map_type_sound with (t := t1).
         + constructor. auto.
-        + intros; repeat apply_type_sound_IH; repeat apply well_formed_locals_step; auto.
+        + intros; repeat apply_type_sound_IH; repeat apply locals_wf_step; auto;
+            try apply_type_of__type_wf; try invert_type_wf; auto.
     Qed.
   End WithMap.
 End WithWord.
